# A szorzatfüggvény deriválási szabálya

## Kimondás
Tegyük fel, hogy $f,g \in \R \to \R$ és $f,g \in D\{a\}$ valamilyen $a \in \ int (\mathcal{D}_f \cap \mathcal{D}_g)$ pontban.\
Ekkor

$$f \cdot g \in D\{a\} \\ \mathrm{és} \\ \left(f \cdot g \right)^{\prime}(a) = f^{\prime}(a)g(a) + f(a)g^{\prime}(a)$$

## Bizonyítás
Nyilván $a \in \ int \ \mathcal{D}_{fg}$, hiszen $\mathcal{D}_{fg} = \mathcal{D}_f \cap \mathcal{D}_g$. Másrészt
$$(fg)^{\prime}(a) = \lim_{x \to a}{\frac{(fg)(x) - (fg)(a)}{x-a}} = \lim_{x \to a}{\frac{f(x)g(x) - f(a)g(a)}{x-a}} =$$
$$= \lim_{x \to a}{\frac{f(x)g(x)-f(a)g(x)+f(a)g(x)-f(a)g(a)}{x-a}} = $$
$$= \lim_{x \to a}{\frac{(f(x)-f(a))g(x) + f(a)(g(x)-g(a))}{x-a}} = $$
$$= \lim_{x \to a}{\frac{f(x)-f(a)}{x-a}}\lim_{x \to a}{g(x)+f(a)}\lim_{x \to a}{\frac{g(x)-g(a)}{x-a}} = f^{\prime}(a)g(a)+f(a)g^{\prime}(a)$$